put index directly on coxeterMove definition

DemazureOperators/Matsumoto.lean
@@ -6,71 +6,77 @@ variable {W : Type} [Group W] [DecidableEq W]
 variable {M : CoxeterMatrix B} (cs : CoxeterSystem M W)
 
 inductive CoxeterMove (cs : CoxeterSystem M W) where
-| nil (i : B) : CoxeterMove cs
-| braid (i j : B) : CoxeterMove cs
+| nil (i : B) (p : ℕ) : CoxeterMove cs
+| braid (i j : B) (p : ℕ) : CoxeterMove cs
 
 def apply_coxeterMove (s : CoxeterMove cs) (l : List B) : List B :=
   match s with
-  | CoxeterMove.nil i =>
-    if l.take 2 = [i, i] then
-      l.drop 2
-    else
-      l
-  | CoxeterMove.braid i j =>
-    if l.take (M i j) = braidWord M i j then
-      braidWord M i j ++ l.drop (M i j)
-    else
-      l
+  | CoxeterMove.nil i p =>
+    match p with
+    | 0 =>
+      if l.take 2 = [i, i] then
+        l.drop 2
+      else
+        l
+    | p + 1 =>
+      match l with
+      | [] => []
+      | h::t => h :: apply_coxeterMove (CoxeterMove.nil i p) t
+
+  | CoxeterMove.braid i j p =>
+    match p with
+    | 0 =>
+      if l.take (M i j) = braidWord M i j then
+        braidWord M i j ++ l.drop (M i j)
+      else
+        l
+    | p + 1 =>
+      match l with
+      | [] => []
+      | h::t => h :: apply_coxeterMove (CoxeterMove.braid i j p) t
 
 local prefix:100 "s" => cs.simple
 local prefix:100 "π" => cs.wordProd
 local prefix:100 "ℓ" => cs.length
 
 theorem coxeterMove_wordProd (cm : CoxeterMove cs) (l : List B) : π (apply_coxeterMove cs cm l) = π l := by
-  simp [apply_coxeterMove]
   cases cm with
-  | nil i =>
-    simp
-    by_cases h : l.take 2 = [i, i]
-    · simp[h]
-      have h' : l = l.take 2 ++ l.drop 2 := by simp
-      nth_rewrite 2 [h']
-      rw[wordProd_append]
-      rw[h]
-      simp
-      convert_to cs.wordProd ([i] ++ [i]) = 1
-      rw[wordProd_append]
-      simp
-    · simp[h]
-  | braid i j =>
-    simp
-    by_cases h : List.take (M.M i j) l = braidWord M i j
-    · simp[h]
-      have h' : l = l.take (M.M i j) ++ l.drop (M.M i j) := by simp
-      nth_rewrite 2 [h']
-      repeat rw[wordProd_append]
-      rw[h]
-    · simp[h]
+  | nil i p =>
+    match p with
+    | 0 =>
+      simp[apply_coxeterMove]
+      by_cases h : l.take 2 = [i, i]
+      · simp[h]
+        have h' : l = l.take 2 ++ l.drop 2 := by simp
+        nth_rewrite 2 [h']
+        rw[wordProd_append]
+        rw[h]
+        simp
+        convert_to cs.wordProd ([i] ++ [i]) = 1
+        rw[wordProd_append]
+        simp
+      · simp[h]
+    | p + 1 =>
+      match l with
+      | [] => simp[apply_coxeterMove]
+      | h::t =>
+        simp[apply_coxeterMove, wordProd_cons]
+        exact coxeterMove_wordProd (CoxeterMove.nil i p) t
 
-
-def apply_coxeterMove_atIndex (cm : CoxeterMove cs) (l : List B) (p : ℕ) : List B :=
-  match p with
-  | 0 => apply_coxeterMove cs cm l
-  | p + 1 => match l with
-    | [] => []
-    | h::t => h :: apply_coxeterMove_atIndex cm t p
-
-theorem coxeterMove_atIndex_wordProd (cm : CoxeterMove cs) (p : ℕ) (l : List B) : π (apply_coxeterMove_atIndex cs cm l p) = π l := by
-  revert l
-  induction p with
-  | zero =>
-    intro l
-    simp[apply_coxeterMove_atIndex]
-    rw[coxeterMove_wordProd]
-  | succ p ih =>
-    intro l
-    match l with
-    | [] => simp[apply_coxeterMove_atIndex]
-    | h::t =>
-      simp[apply_coxeterMove_atIndex, wordProd_cons]
-      exact ih t
+  | braid i j p =>
+    match p with
+    | 0 =>
+      simp[apply_coxeterMove]
+      by_cases h : List.take (M.M i j) l = braidWord M i j
+      · simp[h]
+        have h' : l = l.take (M.M i j) ++ l.drop (M.M i j) := by simp
+        nth_rewrite 2 [h']
+        repeat rw[wordProd_append]
+        rw[h]
+      · simp[h]
+    | p + 1 =>
+      match l with
+      | [] => simp[apply_coxeterMove]
+      | h::t =>
+        simp[apply_coxeterMove, wordProd_cons]
+        exact coxeterMove_wordProd (CoxeterMove.braid i j p) t
